pweq fun checkpoint

theories/diffpriv/examples/exact_cache.v
@@ -193,26 +193,45 @@ Section xcache.
              "v"
           end).
 
+
+  (* we can define the original exact_cache as a client of the online spec (keeping the direct def.) *)
+  Definition exact_cache_offline : val :=
+    λ:"M" "qs" "db",
+      let: "oXC" := online_xcache "M" "db" in
+      list_fold (λ: "acc" "q", list_cons ("oXC" "q") "acc") list_nil "qs".
+
+  (* same but with list_map *)
+  Definition exact_cache_offline_map : val :=
+    λ:"M" "qs" "db",
+      let: "oXC" := online_xcache "M" "db" in
+      list_map "oXC" "qs".
+
+  Definition oxc_spec0_cached (f f' : val) (F : gmap nat val → iProp Σ) : iProp Σ :=
+    (∀ (q : nat) A K,
+          ⌜q ∈ dom A⌝ -∗
+          F(A) -∗
+          ⤇ fill K (Val f' #q) -∗
+          WP (Val f) #q {{ v, F(A) ∗ ⤇ fill K (Val v) ∗  ⌜A !! q = Some v⌝ }}).
+
+  Definition oxc_spec0_fresh (M : val) c `(dDB : Distance DB) (f f' : val) (F : gmap nat val → iProp Σ) : iProp Σ :=
+    (∀ (q : nat) A ε δ K,
+          ⌜q ∉ dom A⌝ -∗
+          wp_diffpriv (M #q) ε δ dDB -∗
+          ↯m (c * ε) -∗
+          ↯ (c * δ) -∗
+          F(A) -∗
+          ⤇ fill K (Val f' #q) -∗
+          WP (Val f) #q {{ v, F( <[q := v]> A) ∗ ⤇ fill K (Val v) ∗ ⌜<[q := v]> A !! q = Some v⌝ }}).
+
   (* pay as you go, cache map exposed, M only needs to be private on the queries it gets executed on *)
-  Lemma oxc_spec0 (M : val) `(dDB : Distance DB) (db db' : DB) (adj : dDB db db' <= 1) K :
+  Lemma oxc_spec0 (M : val) `(dDB : Distance DB) (db db' : DB) c (adj : dDB db db' <= c) K :
     ⤇ fill K (online_xcache M (Val (inject db')))
     ⊢ WP online_xcache M (Val (inject db))
         {{ f, ∃ f', ⤇ fill K (Val f') ∗
               ∃ (F : gmap nat val → iProp Σ),
               F ∅ ∗
-              (∀ (q : nat) A K,
-                  ⌜q ∈ dom A⌝ -∗
-                  F(A) -∗
-                  ⤇ fill K (Val f' #q) -∗
-                  WP (Val f) #q {{ v, F(A) ∗ ⤇ fill K (Val v) ∗  ⌜A !! q = Some v⌝ }}) ∗
-              (∀ (q : nat) A ε δ K,
-                  ⌜q ∉ dom A⌝ -∗
-                  wp_diffpriv (M #q) ε δ dDB -∗
-                  ↯m ε -∗
-                  ↯ δ -∗
-                  F(A) -∗
-                  ⤇ fill K (Val f' #q) -∗
-                  WP (Val f) #q {{ v, F( <[q := v]> A) ∗ ⤇ fill K (Val v) ∗ ⌜<[q := v]> A !! q = Some v⌝ }})
+              □ oxc_spec0_cached f f' F ∗
+              □ oxc_spec0_fresh M c dDB f f' F
         }}.
   Proof.
     iIntros "rhs".
@@ -226,7 +245,7 @@ Section xcache.
     iExists (λ A, map_list cache_l A ∗ map_slist cache_r A)%I.
     iFrame.
     iSplitR.
-    - iIntros (??? cached) "[cache_l cache_r] rhs". tp_pures. wp_pures.
+    - iIntros "!>" (??? cached) "[cache_l cache_r] rhs". tp_pures. wp_pures.
       tp_bind (get _ _).
       iMod (spec_get with "[$cache_r] [$rhs]") as "[rhs cache_r]".
       wp_apply (wp_get with "cache_l") ; iIntros (vq) "[cache_l %hvq]".
@@ -234,7 +253,7 @@ Section xcache.
       apply elem_of_dom in cached. rewrite /opt_to_val.
       destruct cached as [vq hvq]. rewrite hvq.
       tp_pures. wp_pures. iFrame. done.
-    - iIntros (????? cached) "M_dipr ε δ [cache_l cache_r] rhs". tp_pures. wp_pures.
+    - iIntros "!>" (????? cached) "M_dipr ε δ [cache_l cache_r] rhs". tp_pures. wp_pures.
       tp_bind (get _ _).
       iMod (spec_get with "[$cache_r] [$rhs]") as "[rhs cache_r]".
       wp_apply (wp_get with "cache_l") ; iIntros (vq) "[cache_l %hvq]".
@@ -242,8 +261,7 @@ Section xcache.
       apply not_elem_of_dom_1 in cached. rewrite /opt_to_val.
       rewrite !cached. tp_pures ; wp_pures.
       tp_bind (M _ _). wp_bind (M _ _).
-      rewrite /wp_diffpriv. iSpecialize ("M_dipr" $! _ 1 db db' adj).
-      rewrite !Rmult_1_l.
+      rewrite /wp_diffpriv. iSpecialize ("M_dipr" $! _ c db db' adj).
       iSpecialize ("M_dipr" with "[$rhs $ε $δ]").
       iPoseProof (wp_frame_l with "[cache_r $M_dipr]") as "M_dipr". 1: iAssumption.
       iPoseProof (wp_frame_l with "[cache_l $M_dipr]") as "M_dipr". 1: iAssumption.
@@ -254,70 +272,936 @@ Section xcache.
       simpl. tp_pures. wp_pures. iFrame. iPureIntro. by rewrite lookup_insert.
   Qed.
 
-  (* F can store error credits ; could also ask for N*ε error credits upfront and hand out F(∅, N) instead of F(∅, 0). *)
-  Lemma oxc_spec1 (M : val) `(dDB : Distance DB) (db db' : DB) (adj : dDB db db' <= 1) K ε δ (εpos : 0 <= ε) (δpos : 0 <= δ) :
-    (∀ q : nat, hoare_diffpriv (M #q) ε δ dDB) ∗
+  Definition oxc_spec0_pw_cached (f f' : val) (G : gmap nat val → gmap nat val → iProp Σ) : iProp Σ :=
+    (∀ (q : nat) B B' K,
+          ⌜q ∈ dom B⌝ -∗
+          ⌜q ∈ dom B'⌝ -∗
+          G B B' -∗
+          ⤇ fill K (Val f' #q) -∗
+          WP (Val f) #q {{ v, ∃ v' : val, G B B' ∗ ⤇ fill K (Val v') ∗
+                                          ⌜B !! q = Some v⌝ ∗ ⌜B' !! q = Some v'⌝ ∗
+                                          ⌜B = B' → v = v'⌝ }}).
+
+  Definition oxc_spec0_pw_fresh (M : val) c `(dDB : Distance DB) (f f' : val) (F : gmap nat val → iProp Σ)
+    (G : gmap nat val → gmap nat val → iProp Σ)
+    : iProp Σ :=
+    (∀ (q : nat) B B' ε δ K,
+        ⌜q ∉ dom B⌝ -∗
+        ⌜q ∉ dom B'⌝ -∗
+        wp_diffpriv_pw (M #q) ε δ dDB -∗
+        ↯m (c * ε) -∗
+        ↯ (c * δ) -∗
+        G B B' -∗
+        ⤇ fill K (Val f' #q) -∗
+        ∀ RES,
+          (* WP (Val f) #q {{ v, ∃ (v' : val) A', F A' ∗ ⤇ fill K (Val v') ∗ ⌜v = RES → (v' = RES ∧ A' = <[q := v]> A)⌝ }}). *)
+          WP (Val f) #q {{ v, ∃ (v' : val),
+                  G ((<[q := v]> B)) (<[q := v']> B') ∗
+                  ⤇ fill K (Val v') ∗
+                  (⌜v = RES ∧ B = B'⌝ -∗ G ((<[q := v]> B)) (<[q := v']> B') -∗ F (<[q := v]> B) ∗ ⌜(v' = RES)⌝) }}).
+          (* WP (Val f) #q {{ v, ⌜v = RES⌝ -∗ F( <[q := v]> A) ∗ ⤇ fill K (Val v) ∗ ⌜<[q := v]> A !! q = Some v⌝ }}). *)
+
+  (* pointwise equality variant *)
+  Lemma oxc_spec0_pw (M : val) `(dDB : Distance DB) (db db' : DB) `(adj : dDB db db' <= c) K :
     ⤇ fill K (online_xcache M (Val (inject db')))
     ⊢ WP online_xcache M (Val (inject db))
         {{ f, ∃ f', ⤇ fill K (Val f') ∗
-              ∃ (F : gmap nat val * nat → iProp Σ),
-              F (∅, 0%nat) ∗
-              (∀ A k, ↯m ε ∗ ↯ δ ∗ F(A, k) -∗ F(A, S k)) ∗
-              (∀ (q : nat) A K (N : nat),
-                  ⌜q ∈ dom A⌝ -∗
-                  F(A, N) -∗
-                  ⤇ fill K (Val f' #q) -∗
-                  WP (Val f) #q {{ v, F(A, N) ∗ ⤇ fill K (Val v) ∗  ⌜A !! q = Some v⌝ }}) ∗
-              (∀ (q : nat) A K (N : nat),
-                  ⌜q ∉ dom A⌝ -∗
-                  F(A, S N) -∗
-                  ⤇ fill K (Val f' #q) -∗
-                  WP (Val f) #q {{ v, F( <[q := v]> A, N) ∗ ⤇ fill K (Val v) ∗ ⌜<[q := v]> A !! q = Some v⌝ }})
+              ∃ (F : gmap nat val → iProp Σ) (G : gmap nat val → gmap nat val → iProp Σ),
+              F ∅ ∗ □ (∀ A, F A ∗-∗ G A A) ∗
+              □ oxc_spec0_pw_cached f f' G ∗
+              □ oxc_spec0_pw_fresh M c dDB f f' F G
         }}.
   Proof.
-    iIntros "(#M_dipr & rhs)".
-    unshelve iPoseProof (oxc_spec0 with "[rhs]") as "spec0" => //.
-    iMod ecm_zero as "ε0".
-    iMod ec_zero as "δ0".
-    iPoseProof (wp_frame_l with "[ε0 δ0 $spec0]") as "spec0". 1: iApply (combine_sep_as with "[ε0 δ0]").
-    2: iSplitR "δ0". 2: iApply "ε0". 2: iApply "δ0". 1: done.
-    iPoseProof (wp_frame_l with "[M_dipr $spec0]") as "spec0". 1: iApply "M_dipr".
-    iApply (wp_mono with "spec0").
-    iIntros "%f (#M_dipr & (ε0 & δ0) & %f' & rhs & (%F & F0 & f_cached & f_fresh))".
-    iExists f'. iFrame "rhs".
-    iExists (λ Ak : gmap nat val * nat, let (A, k) := Ak in F A ∗ ↯m (k * ε) ∗ ↯ (k * δ))%I.
-    rewrite !Rmult_0_l. iFrame "F0 ε0 δ0".
-    iSplitR ; [|iSplitL "f_cached"].
-    - iIntros (??) "(ε&δ&?&kε&kδ)". iFrame. iPoseProof (ecm_combine with "[ε kε]") as "ε" ; iFrame.
-      iPoseProof (ec_combine with "[δ kδ]") as "δ" ; iFrame. iSplitL "ε".
-      + iApply ecm_eq. 2: iFrame. replace (S k) with (k+1)%nat by lia. replace (INR (k+1)) with (k+1)%R.
-        2: real_solver. lra.
-      + iApply ec_eq. 2: iFrame. replace (S k) with (k+1)%nat by lia. replace (INR (k+1)) with (k+1)%R.
-        2: real_solver. lra.
-    - simpl. iIntros (?????) "[FA [ε δ]] rhs".
-      iSpecialize ("f_cached" with "[] [$FA] [$rhs]") => //.
-      iPoseProof (wp_frame_l with "[$f_cached ε δ]") as "f_cached".
-      1: iApply (combine_sep_as with "[ε δ]").
-      2: iSplitR "δ". 2: iApply "ε". 2: iApply "δ". 1: done.
-      iApply (wp_mono with "f_cached"). iIntros (?) "((ε & δ) & FA & rhs & %)". iFrame => //.
-    - iIntros (?????) "[FA [ε δ]] rhs".
-      replace ((S N)) with (N + 1)%nat by lia. replace (INR (N+1)) with (N+1) by real_solver.
-      rewrite !Rmult_plus_distr_r. rewrite !Rmult_1_l.
-      iDestruct (ecm_split with "ε") as "[Nε ε]". 1,2: real_solver.
-      iDestruct (ec_split with "δ") as "[Nδ δ]". 1,2: real_solver.
-      iSpecialize ("f_fresh" with "[] [] [$ε] [$δ] [$FA] [$rhs]") => //.
-      { iIntros (?????) "[??]". iApply ("M_dipr" with "[] [-]") => //. 2: iNext ; iIntros => //.
-        iFrame. }
-      iPoseProof (wp_frame_l with "[$f_fresh Nε Nδ]") as "f_fresh".
-      1: iApply (combine_sep_as with "[Nε Nδ]").
-      2: iSplitR "Nδ". 2: iApply "Nε". 2: iApply "Nδ". 1: done.
-      iApply (wp_mono with "f_fresh"). iIntros (?) "((ε & δ) & FA & rhs & %)". iFrame => //.
+    iIntros "rhs".
+    rewrite /online_xcache. wp_pures.
+    tp_pures. tp_bind (init_map _). iMod (spec_init_map with "rhs") as "[%cache_r [rhs cache_r]]".
+    simpl. tp_pures.
+    wp_apply wp_init_map => //. iIntros (cache_l) "?". wp_pures.
+
+    iModIntro. iExists _. simpl. iFrame "rhs".
+
+    iExists (λ A, map_list cache_l A ∗ map_slist cache_r A)%I.
+    iExists (λ B B', map_list cache_l B ∗ map_slist cache_r B')%I.
+    iFrame.
+    repeat iSplitR.
+    - iModIntro. iIntros. iSplit ; by iIntros.
+    - iIntros "!>" (???? cached cached') "[cache_l cache_r] rhs". tp_pures. wp_pures.
+      tp_bind (get _ _).
+      iMod (spec_get with "[$cache_r] [$rhs]") as "[rhs cache_r]".
+      wp_apply (wp_get with "cache_l") ; iIntros (vq) "[cache_l %hvq]".
+      simpl. subst.
+      apply elem_of_dom in cached, cached'. rewrite /opt_to_val.
+      destruct cached as [vq hvq]. rewrite hvq.
+      destruct cached' as [vq' hvq']. rewrite hvq'.
+      tp_pures. wp_pures. iFrame. iModIntro ; iPureIntro ; intuition auto. simplify_eq. done.
+    - iIntros "!>" (?????? cached cached') "M_dipr ε δ [cache_l cache_r] rhs %RES". tp_pures. wp_pures.
+      tp_bind (get _ _).
+      iMod (spec_get with "[$cache_r] [$rhs]") as "[rhs cache_r]".
+      wp_apply (wp_get with "cache_l") ; iIntros (vq) "[cache_l %hvq]".
+      simpl. subst.
+      apply not_elem_of_dom_1 in cached, cached'. rewrite /opt_to_val.
+      rewrite cached cached'. tp_pures ; wp_pures.
+      tp_bind (M _ _). wp_bind (M _ _).
+      rewrite /wp_diffpriv_pw. iSpecialize ("M_dipr" $! _ c db db' adj).
+      (* rewrite !Rmult_1_l. *)
+      iSpecialize ("M_dipr" with "[$rhs $ε $δ]").
+      iSpecialize ("M_dipr" $! RES).
+      iPoseProof (wp_frame_l with "[cache_r $M_dipr]") as "M_dipr". 1: iAssumption.
+      iPoseProof (wp_frame_l with "[cache_l $M_dipr]") as "M_dipr". 1: iAssumption.
+      iApply (wp_mono with "M_dipr").
+      iIntros (vq) "[cache_l [cache_r rhs]]" => /=.
+      iDestruct "rhs" as "(%v' & rhs & %pweq)".
+      tp_pures. wp_pures. tp_bind (set _ _ _). iMod (spec_set with "[$cache_r] [$rhs]") as "[rhs cache_r]".
+      wp_apply (wp_set with "cache_l") ; iIntros "cache_l".
+      simpl. tp_pures. wp_pures. (* iExists v',(<[q:=vq]> A). *)
+      iModIntro. iFrame. iIntros "[->->]". rewrite pweq //.
+      iIntros "[F_l F_r]". iFrame. done.
+      (* iFrame. iPureIntro. by rewrite lookup_insert. *)
   Qed.
 
+  (* BEGIN TEMP COMMENT *)
+  (* (* F can store error credits ; could also ask for N*ε error credits upfront and hand out F(∅, N) instead of F(∅, 0). *)
+     Lemma oxc_spec1 (M : val) `(dDB : Distance DB) (db db' : DB) (adj : dDB db db' <= 1) K ε δ (εpos : 0 <= ε) (δpos : 0 <= δ) :
+       (∀ q : nat, hoare_diffpriv (M #q) ε δ dDB) ∗
+       ⤇ fill K (online_xcache M (Val (inject db')))
+       ⊢ WP online_xcache M (Val (inject db))
+           {{ f, ∃ f', ⤇ fill K (Val f') ∗
+                 ∃ (F : gmap nat val * nat → iProp Σ),
+                 F (∅, 0%nat) ∗
+                 (∀ A k, ↯m ε ∗ ↯ δ ∗ F(A, k) -∗ F(A, S k)) ∗
+                 (∀ (q : nat) A K (N : nat),
+                     ⌜q ∈ dom A⌝ -∗
+                     F(A, N) -∗
+                     ⤇ fill K (Val f' #q) -∗
+                     WP (Val f) #q {{ v, F(A, N) ∗ ⤇ fill K (Val v) ∗  ⌜A !! q = Some v⌝ }}) ∗
+                 (∀ (q : nat) A K (N : nat),
+                     ⌜q ∉ dom A⌝ -∗
+                     F(A, S N) -∗
+                     ⤇ fill K (Val f' #q) -∗
+                     WP (Val f) #q {{ v, F( <[q := v]> A, N) ∗ ⤇ fill K (Val v) ∗ ⌜<[q := v]> A !! q = Some v⌝ }})
+           }}.
+     Proof.
+       iIntros "(#M_dipr & rhs)".
+       unshelve iPoseProof (oxc_spec0 with "[rhs]") as "spec0" => //.
+       iMod ecm_zero as "ε0".
+       iMod ec_zero as "δ0".
+       iPoseProof (wp_frame_l with "[ε0 δ0 $spec0]") as "spec0". 1: iApply (combine_sep_as with "[ε0 δ0]").
+       2: iSplitR "δ0". 2: iApply "ε0". 2: iApply "δ0". 1: done.
+       iPoseProof (wp_frame_l with "[M_dipr $spec0]") as "spec0". 1: iApply "M_dipr".
+       iApply (wp_mono with "spec0").
+       iIntros "%f (#M_dipr & (ε0 & δ0) & %f' & rhs & (%F & F0 & f_cached & f_fresh))".
+       iExists f'. iFrame "rhs".
+       iExists (λ Ak : gmap nat val * nat, let (A, k) := Ak in F A ∗ ↯m (k * ε) ∗ ↯ (k * δ))%I.
+       rewrite !Rmult_0_l. iFrame "F0 ε0 δ0".
+       iSplitR ; [|iSplitL "f_cached"].
+       - iIntros (??) "(ε&δ&?&kε&kδ)". iFrame. iPoseProof (ecm_combine with "[ε kε]") as "ε" ; iFrame.
+         iPoseProof (ec_combine with "[δ kδ]") as "δ" ; iFrame. iSplitL "ε".
+         + iApply ecm_eq. 2: iFrame. replace (S k) with (k+1)%nat by lia. replace (INR (k+1)) with (k+1)%R.
+           2: real_solver. lra.
+         + iApply ec_eq. 2: iFrame. replace (S k) with (k+1)%nat by lia. replace (INR (k+1)) with (k+1)%R.
+           2: real_solver. lra.
+       - simpl. iIntros (?????) "[FA [ε δ]] rhs".
+         iSpecialize ("f_cached" with "[] [$FA] [$rhs]") => //.
+         iPoseProof (wp_frame_l with "[$f_cached ε δ]") as "f_cached".
+         1: iApply (combine_sep_as with "[ε δ]").
+         2: iSplitR "δ". 2: iApply "ε". 2: iApply "δ". 1: done.
+         iApply (wp_mono with "f_cached"). iIntros (?) "((ε & δ) & FA & rhs & %)". iFrame => //.
+       - iIntros (?????) "[FA [ε δ]] rhs".
+         replace ((S N)) with (N + 1)%nat by lia. replace (INR (N+1)) with (N+1) by real_solver.
+         rewrite !Rmult_plus_distr_r. rewrite !Rmult_1_l.
+         iDestruct (ecm_split with "ε") as "[Nε ε]". 1,2: real_solver.
+         iDestruct (ec_split with "δ") as "[Nδ δ]". 1,2: real_solver.
+         iSpecialize ("f_fresh" with "[] [] [ε] [δ] [$FA] [$rhs]") => //.
+         { iIntros (?????) "[??]". iApply ("M_dipr" with "[] [-]") => //. 2: iNext ; iIntros => //.
+           iFrame. }
+         1,2: rewrite Rmult_1_l => //.
+         iPoseProof (wp_frame_l with "[$f_fresh Nε Nδ]") as "f_fresh".
+         1: iApply (combine_sep_as with "[Nε Nδ]").
+         2: iSplitR "Nδ". 2: iApply "Nε". 2: iApply "Nδ". 1: done.
+         iApply (wp_mono with "f_fresh"). iIntros (?) "((ε & δ) & FA & rhs & %)". iFrame => //.
+     Qed.
 
-  (* TODO define the original exact_cache as a client of the online spec (keeping the direct def.) *)
-  (* TODO prove exact_cache_dipr from the online spec *)
+     (* we can prove exact_cache_dipr from the online spec *)
+     Lemma exact_cache_dipr_offline (M : val) DB (dDB : Distance DB) (qs : list nat) (QS : val) (is_qs : is_list qs QS)
+       ε δ (εpos : 0 <= ε) (δpos : 0 <= δ)
+       (M_dipr : Forall (λ q : nat, ⊢ wp_diffpriv (M #q) ε δ dDB) qs)
+       :
+       let k := size ((list_to_set qs) : gset _) in
+       ⊢ wp_diffpriv (exact_cache_offline M QS) (k*ε) (k*δ) dDB.
+     Proof with (tp_pures ; wp_pures).
+       iIntros (k K c db db' adj) "[rhs [ε δ]]".
+       rewrite {2}/exact_cache_offline...
+       rewrite /exact_cache_offline...
+       tp_bind (online_xcache _ _). wp_bind (online_xcache _ _).
+       iPoseProof (oxc_spec0 M _ _ _ _) as "oXC" => //.
+       iSpecialize ("oXC" with "rhs").
+       iApply (wp_strong_mono'' with "oXC").
+       iIntros "%f (%f' & rhs & %F & F & #cached & #fresh) /="...
+       set (exact_cache_offline_body (f : val) := (λ: "acc" "q", list_cons (f "q") "acc")%V).
+       rewrite -!/(exact_cache_offline_body _).
+       revert qs QS is_qs k M_dipr.
+       cut
+         (∀ (qs : list nat)
+            (qs_pre qs' : list nat) (QS' : val)
+            (acc : val) cache_map,
+             qs = qs_pre ++ qs' →
+             dom cache_map = list_to_set qs_pre →
+             dom cache_map ∪ list_to_set qs' = list_to_set qs →
+             is_list qs' QS' →
+             Forall (λ q : nat, ⊢ wp_diffpriv (M #q) ε δ dDB) qs →
+             let k := size (list_to_set qs : gset nat) in
+             let k' := size cache_map in
+             {{{
+                   ↯m (c * ((k - k') * ε)) ∗ ↯ (c * ((k - k') * δ)) ∗
+                   □ oxc_spec0_cached f f' F ∗
+                   □ oxc_spec0_fresh M c dDB f f' F ∗
+                   ⤇ fill K (list_fold (exact_cache_offline_body f') acc QS') ∗
+                   F cache_map
+             }}}
+               list_fold (exact_cache_offline_body f) acc QS'
+               {{{ vl, RET vl ; ∃ (vr : val), ⤇ fill K vr ∗ ⌜vl = vr⌝ }}}
+         ).
+       {
+         intros h. intros. iApply (h qs [] qs QS _ ∅ with "[-]") => //.
+         1: set_solver.
+         2: iNext ; iIntros (?) "(% & ? & ->)" ; done.
+         iFrame. rewrite map_size_empty. rewrite Rminus_0_r. subst k. simpl. iFrame.
+         iSplit ; done.
+       }
+       iLöb as "IH".
+       iIntros (qs qs_pre qs' QS' acc cache qs_pre_qs' dom_cache_pre dom_cache_qs'_qs is_qs'
+                  M_dipr φ) "(ε & δ & #cached & #fresh & rhs & F) hφ".
+       set (k := size (list_to_set qs : gset nat)).
+       set (k' := size cache).
+       rewrite {4}/exact_cache_offline_body/list_fold... rewrite -!/(exact_cache_offline_body _) -/list_fold.
+       destruct qs' as [|q' qs''] eqn:qs'_qs''.
+       1:{ rewrite is_qs'. rewrite {3}/exact_cache_offline_body/list_fold... iApply "hφ". iExists _. iFrame => //. }
+       destruct is_qs' as (QS'' & -> & is_qs'')...
+       rewrite -!/(exact_cache_offline_body _) -/list_fold.
+       rewrite qs_pre_qs' in M_dipr.
+       destruct ((proj1 (List.Forall_app _ _ _)) M_dipr) as [M_dipr_qs_pre M_dipr_qs'].
+       destruct (Forall_cons_1 _ _ _ M_dipr_qs') as [M_dipr_q' M_dipr_qs''].
+       assert (0 <= dDB db db') by apply distance_pos.
+       destruct (cache !! q') eqn:cache_q' => /=.
+       - opose proof (elem_of_dom_2 _ _ _ cache_q') as h...
+         rewrite /exact_cache_offline_body...
+         tp_bind (f' _) ; wp_bind (f _).
+         iCombine "cached" as "h".
+         iSpecialize ("h" $! q' cache _ h with "F rhs").
+         iApply (wp_strong_mono'' with "h").
+         iIntros "/= %v' (F & rhs & %cache_q'')".
+         assert (v = v') as <-. { rewrite cache_q' in cache_q''. inversion cache_q''. done. }
+         rewrite /list_cons...
+         rewrite -!/(exact_cache_offline_body _) -/list_fold.
+         iSpecialize ("IH" $! qs (qs_pre ++ [q']) qs'' QS'' (InjRV (v, acc)) cache).
+         unshelve iApply ("IH" $! _ _ _ _ _ _ with "[ε δ rhs F]") => //.
+         1: subst ; by rewrite cons_middle assoc.
+         all: subst ; try assumption.
+         1,2: set_solver. iFrame. iSplit ; done.
+       - opose proof (not_elem_of_dom_2 _ _ cache_q') as h...
+         assert ((c * ((k - k') * ε)) = (c * (k - (k'+1)) * ε + c * ε)) as -> by lra.
+         assert ((c * ((k - k') * δ)) = (c * (k - (k'+1)) * δ + c * δ)) as -> by lra.
+         assert (0 <= k - (k' + 1)).
+         {
+           subst. subst k k'. apply Rle_0_le_minus.
+           rewrite -dom_cache_qs'_qs.
+           replace (size cache) with (size (dom cache)) by apply size_dom.
+           rewrite dom_cache_pre.
+           replace 1 with (INR 1) by auto.
+           replace 1%nat with (size (list_to_set [q'] : gset nat)).
+           2:{ cbn. rewrite union_empty_r_L. apply size_singleton. }
+           rewrite -plus_INR.
+           rewrite -size_union.
+           2: set_solver.
+           rewrite (list_to_set_cons _ qs''). simpl.
+           apply le_INR.
+           apply subseteq_size. set_solver.
+         }
+         iDestruct (ecm_split with "ε") as "[kε ε]".
+         2: real_solver. 1: repeat real_solver_partial => //.
+         iDestruct (ec_split with "δ") as "[kδ δ]".
+         2: real_solver. 1: repeat real_solver_partial => //.
+         rewrite /exact_cache_offline_body...
+         tp_bind (f' _) ; wp_bind (f _).
+         iCombine "fresh" as "h".
+         iSpecialize ("h" $! q' cache ε δ _ h M_dipr_q' with "ε δ F rhs").
+         iApply (wp_strong_mono'' with "h").
+         iIntros "/= %vq' (F & rhs & %cache_q'') /=".
+         rewrite /list_cons... rewrite -/list_cons.
+         iSpecialize ("IH" $! qs (qs_pre ++ [q']) qs'' QS'' (InjRV (vq', acc)) _).
+         iSpecialize ("IH" $! _ _ _ _ _ _) => //.
+         iSpecialize ("IH" with "[kε kδ rhs $F]") => //.
+         2: iApply "IH" => //. iFrame.
+         iSplitL "kε" ; [|iSplitL "kδ"]. 3: iSplit ; done.
+         + iApply ecm_eq. 2: iFrame. real_solver_partial.
+           subst k. simpl. subst k'.
+           replace (INR $ size (<[q' := vq']> cache)) with (size cache + 1).
+           1: done.
+           rewrite map_size_insert_None => //. qify_r ; zify_q. lia.
+         + iApply ec_eq. 2: iFrame. real_solver_partial.
+           subst k. simpl. subst k'.
+           replace (INR $ size (<[q' := vq']> cache)) with (size cache + 1).
+           1: done.
+           rewrite map_size_insert_None => //. qify_r ; zify_q. lia.
+           Unshelve.
+           1: subst ; by rewrite cons_middle assoc.
+           all: subst ; assumption || set_solver.
+     Qed.
 
+
+     (* we can prove exact_cache_dipr from the online spec *)
+     Lemma exact_cache_dipr_offline_map (M : val) DB (dDB : Distance DB) (qs : list nat) (QS : val) (is_qs : is_list qs QS)
+       ε δ (εpos : 0 <= ε) (δpos : 0 <= δ)
+       (M_dipr : Forall (λ q : nat, ⊢ wp_diffpriv (M #q) ε δ dDB) qs)
+       :
+       let k := size ((list_to_set qs) : gset _) in
+       ⊢ wp_diffpriv (exact_cache_offline_map M QS) (k*ε) (k*δ) dDB.
+     Proof with (tp_pures ; wp_pures).
+       iIntros (k K c db db' adj) "[rhs [ε δ]]".
+       rewrite {2}/exact_cache_offline_map...
+       rewrite /exact_cache_offline_map...
+       tp_bind (online_xcache _ _). wp_bind (online_xcache _ _).
+       iPoseProof (oxc_spec0 M _ _ _ _) as "oXC" => //.
+       iSpecialize ("oXC" with "rhs").
+       iApply (wp_strong_mono'' with "oXC").
+       iIntros "%f (%f' & rhs & %F & F & #cached & #fresh) /="...
+       (* strengthen the postcondition with the resources for the cache & size information for the credits *)
+       cut
+         ( ∀ K, {{{
+                   ↯m (c * (k * ε)) ∗ ↯ (c * (k * δ)) ∗
+                   □ oxc_spec0_cached f f' F ∗
+                   □ oxc_spec0_fresh M c dDB f f' F ∗
+                   ⤇ fill K (list_map f' QS) ∗
+                   F ∅
+             }}}
+                  list_map f QS
+                  {{{ vl, RET vl ;
+                      ∃ (vr : val) (lvl lvr : list val) cache_qs,
+                        ⌜is_list lvl vl⌝ ∗ ⌜is_list lvr vr⌝ ∗ ⌜dom cache_qs = list_to_set qs⌝ ∗
+                        ⤇ fill K vr ∗
+                        F cache_qs ∗
+                        ⌜vl = vr⌝ }}} ).
+       { intros h. intros. iApply (h ∅ with "[-]") => //.
+         2: iNext ; iIntros (?) "(% & % & % & % & % & % & % & rhs & F & %)" ; subst ; done.
+         iFrame. by repeat iSplit. }
+       iInduction qs as [|q' qs'] "IH" forall (QS is_qs).
+       - iIntros (K' φ). iIntros "(ε & δ & #? & #? & rhs & F) hφ".
+         simpl in is_qs. subst. rewrite /list_map... simplify_eq. iApply "hφ". iFrame. iExists [],[].
+         iPureIntro. intuition auto ; try done.
+       - iIntros (K' φ).
+         iIntros "(ε & δ & #cached & #fresh & rhs & F) hφ".
+         set (qs := q' :: qs').
+         rewrite {4}/list_map... rewrite -/list_map.
+         rewrite {3}/list_map... rewrite -/list_map.
+
+         destruct is_qs as (QS' & -> & is_qs')...
+         destruct (Forall_cons_1 _ _ _ M_dipr) as [M_dipr_q' M_dipr_qs'].
+         assert (0 <= dDB db db') by apply distance_pos.
+         tp_bind (list_map f' _) ; wp_bind (list_map f _).
+         iSpecialize ("IH" $! M_dipr_qs' QS' is_qs' _).
+         destruct_decide (make_decision (q' ∈ qs')) as cache_q'.
+         + subst k.
+           assert (list_to_set qs = list_to_set qs') as ->.
+           { subst qs. simpl. set_solver. }
+           iSpecialize ("IH" with "[-hφ]").
+           { iFrame. iSplit ; done. }
+           iApply ("IH"). iIntros "!> %vl (%vr & %lvl & %lvr & %cache_qs' & %is_vl & %is_vr & %dom_cache_qs' & rhs & F & %eqv)".
+           iSimpl in "rhs"... tp_bind (f' _) ; wp_bind (f _).
+           unshelve iSpecialize ("cached" $! q' cache_qs' _ _ with "F rhs").
+           { rewrite dom_cache_qs'. set_solver. }
+           iApply (wp_strong_mono'' with "cached").
+           iIntros "/= %v' (F & rhs & %cache_q'')".
+           rewrite /list_cons...
+           iApply "hφ". iFrame. iModIntro. iPureIntro. simpl.
+           eexists (v' :: lvl), (v' :: lvr). intuition auto.
+           * simpl. eexists _. intuition auto.
+           * simpl. eexists _. intuition auto.
+           * set_solver.
+           * subst. done.
+         + set (k' := size (list_to_set qs' : gset _)).
+           assert ((k = 1 + k')%nat) as ->.
+           { subst k. simpl list_to_set. rewrite size_union. 1: rewrite size_singleton ; lia. set_solver. }
+           replace (c * ((1 + k')%nat * δ)) with (c * δ + c * (k' * δ)).
+           2:{ real_solver_partial. rewrite plus_INR INR_1. field. }
+           replace (c * ((1 + k')%nat * ε)) with (c * ε + c * (k' * ε)).
+           2:{ real_solver_partial. rewrite plus_INR INR_1. field. }
+           iDestruct (ecm_split with "ε") as "[ε k'ε]".
+           2: real_solver. 1: repeat real_solver_partial => //.
+           iDestruct (ec_split with "δ") as "[δ k'δ]".
+           2: real_solver. 1: repeat real_solver_partial => //.
+           iSpecialize ("IH" with "[-hφ ε δ]").
+           { iFrame. iSplit ; done. }
+           iApply "IH".
+           iIntros "!> %vl (%vr & %lvl & %lvr & %cache_qs' & %is_vl & %is_vr & %dom_cache_qs' & rhs & F & %eqv)".
+           iSimpl in "rhs"... tp_bind (f' _) ; wp_bind (f _).
+           unshelve iSpecialize ("fresh" $! q' cache_qs' ε δ _ _ M_dipr_q' with "ε δ F rhs").
+           { rewrite dom_cache_qs'. set_solver. }
+           iApply (wp_strong_mono'' with "fresh").
+           iIntros "/= %v' (F & rhs & %cache_q'')".
+           rewrite /list_cons...
+           iApply "hφ". iFrame. iModIntro. iPureIntro. simpl.
+           eexists (v' :: lvl), (v' :: lvr). intuition auto.
+           * simpl. eexists _. intuition auto.
+           * simpl. eexists _. intuition auto.
+           * set_solver.
+           * subst. done.
+     Qed.
+
+     Section concrete_example.
+
+       Lemma wp_list_map_safe (f : val) (f_safe : ∀ (x : val), ⊢ WP f x {{_, ⌜True⌝ }})
+         (l : list val) (lv : val) (hl : is_list l lv) :
+         ⊢ WP (list_map f lv) {{_, ⌜True⌝}}.
+       Proof.
+         iInduction l as [ | x xs'] "IH" forall (lv hl) ; simpl in hl ; subst.
+         - rewrite /list_map ; wp_pures. done.
+         - rewrite {2}/list_map.
+           destruct hl as (lv' & -> & hl').
+           do 3 wp_pure. fold list_map. wp_pures.
+           wp_bind (list_map _ _).
+           iSpecialize ("IH" $! lv' hl').
+           iApply (wp_strong_mono'' with "IH").
+           iIntros. rewrite /list_cons ; wp_pures.
+           wp_bind (f _). iApply (wp_strong_mono'' $! (f_safe _)). iIntros. wp_pures. done.
+       Qed.
+
+       Lemma spec_list_map_safe (f' : val) (f'_safe : ∀ K (x : val), ⤇ fill K (f' x) ⊢ spec_update ⊤ (∃ v' : val, ⤇ fill K v'))
+         (l : list val) (lv : val) (hl : is_list l lv) K :
+             (⤇ fill K (list_map f' lv)) ⊢ spec_update ⊤ (∃ v' : val, ⤇ fill K v').
+       Proof.
+         iIntros "rhs".
+         iInduction l as [ | x xs'] "IH" forall (lv hl K) ; simpl in hl ; subst.
+         - rewrite /list_map ; tp_pures. iFrame. done.
+         - rewrite {2}/list_map.
+           destruct hl as (lv' & -> & hl').
+           do 3 tp_pure. fold list_map. tp_pures.
+           tp_bind (list_map _ _).
+           iSpecialize ("IH" $! lv' hl').
+           iMod ("IH" with "rhs") as "(% & rhs) /=".
+           rewrite /list_cons ; tp_pures.
+           tp_bind (f' _). iMod (f'_safe with "rhs") as "(% & rhs) /=". tp_pures. iFrame. done.
+       Qed.
+
+       (* An exercise on point-wise equality of lists. *)
+       Variable (f f' : val).
+       (* f and f' are pointwise equal and safe to execute. *)
+       Variable (ff_pweq : ∀ K (x r : val), ⤇ fill K (f' x) ⊢ WP f x {{v , ∃ v' : val, ⤇ fill K v' ∗ ⌜v = r → v' = r⌝ }} ).
+       Variable (f_safe : ∀ x : val, ⊢ WP f x {{ v , ⌜True⌝ }}).
+       Variable (f'_safe : ∀ K (x : val), ⤇ fill K (f' x) ⊢ spec_update ⊤ (∃ v' : val, ⤇ fill K v')).
+
+       (* (map f [0]) and (map f' [0]) are point-wise equal. *)
+       Goal (∀ R, ⊢ ⤇ fill [] (list_map f' (list_cons #0 list_nil)) -∗ WP (list_map f (list_cons #0 list_nil))
+            {{ v , ∃ v' : val , ⤇ fill [] (Val v') ∗ ⌜v = R → v' = R⌝ }}).
+         iIntros "%RES rhs". rewrite /list_map/list_cons. tp_pures. wp_pures.
+         tp_bind (f' _). wp_bind (f _).
+         destruct_decide (make_decision (∃ r0 : val, RES = InjRV (r0, InjLV #()))) as HRES.
+         - destruct HRES as [r0 ->].
+           iPoseProof (ff_pweq _ #0 r0) as "h0".
+           iSpecialize ("h0" with "rhs").
+           iApply (wp_strong_mono'' with "h0").
+           iIntros "%v (%v' & rhs & %hvv') /=". tp_pures. wp_pures.
+           iFrame. iModIntro. iPureIntro. intros h.
+           inversion h. rewrite hvv'. 1: reflexivity. assumption.
+         - iApply (wp_strong_mono'' $! (f_safe _)). iIntros.
+           iMod (f'_safe with "rhs") as "(%v' & rhs)". simpl. tp_pures. wp_pures.
+           iModIntro. iFrame. iPureIntro. intros.
+           exfalso. apply HRES. eauto.
+       Qed.
+
+       (* (map f [1; 0]) and (map f' [1; 0]) are point-wise equal. *)
+       Goal (∀ R, ⊢ ⤇ fill [] (list_map f' (list_cons #1 (list_cons #0 list_nil))) -∗ WP (list_map f (list_cons #1 (list_cons #0 list_nil)))
+            {{ v , ∃ v' : val , ⤇ fill [] (Val v') ∗ ⌜v = R → v' = R⌝ }}).
+
+         iIntros "%RES rhs". rewrite /list_map/list_cons. tp_pures. wp_pures.
+         destruct_decide (make_decision (∃ r1 r0 : val, RES = InjRV (r1, InjRV (r0, InjLV #())))) as HRES.
+         - tp_bind (f' _). wp_bind (f _).
+           destruct HRES as (r1 & r0 & ->).
+           iPoseProof (ff_pweq _ #0 r0) as "h0".
+           iSpecialize ("h0" with "rhs").
+           iApply (wp_strong_mono'' with "h0").
+           iIntros "%v0 (%v0' & rhs & %hvv0') /=". tp_pures. wp_pures.
+
+           tp_bind (f' _). wp_bind (f _).
+           iPoseProof (ff_pweq _ #1 r1) as "h1".
+           iSpecialize ("h1" with "rhs").
+           iApply (wp_strong_mono'' with "h1").
+           iIntros "%v1 (%v1' & rhs & %hvv1') /=". tp_pures. wp_pures.
+
+           iFrame. iModIntro. iPureIntro. intros h.
+           simplify_eq.
+           specialize (hvv0' eq_refl). specialize (hvv1' eq_refl).
+           simplify_eq. reflexivity.
+         - tp_bind (f' _). wp_bind (f _).
+           iApply (wp_strong_mono'' $! (f_safe _)). iIntros.
+           iMod (f'_safe with "rhs") as "(% & rhs)". simpl. tp_pures. wp_pures.
+           tp_bind (f' _). wp_bind (f _).
+           iApply (wp_strong_mono'' $! (f_safe _)). iIntros.
+           iMod (f'_safe with "rhs") as "(% & rhs)". simpl. tp_pures. wp_pures.
+           iModIntro. iFrame. iPureIntro. intros.
+           exfalso. apply HRES. eauto.
+       Qed.
+
+
+
+       (* (map f qs) and (map f' qs) are point-wise equal for any list qs. *)
+       (* This proof reconstructs the entire list of results, which turns out to be overly complicated. *)
+       Goal (∀ K RES (qs : val) QS (hqs : is_list QS qs), ⊢ ⤇ fill K (list_map f' qs) -∗
+                  WP (list_map f qs)
+                    {{ v , ∃ v' : val , ⤇ fill K (Val v') ∗ ⌜v = RES → v' = RES⌝ }}).
+
+         intros. iIntros "rhs".
+         (* we have to conjure up the intermediate results that got collected into RES *)
+         destruct_decide (make_decision (∃ LRES : list val, is_list LRES RES ∧ length LRES = length QS)) as HRES.
+         - destruct HRES as (LRES & hres & res_qs).
+           iInduction QS as [ | Q QS'] "IH" forall (RES LRES res_qs hres qs hqs K) ; simpl in hqs.
+           + subst. rewrite /list_map. tp_pures ; wp_pures. iFrame. done.
+           + destruct hqs as (qs' & hqs & hqs').
+             rewrite {4}/list_map. wp_pures.
+             rewrite hqs.
+             do 4 wp_pure _. fold list_map.
+             destruct LRES as [|RQ LRES']. 1: done.
+             simpl in hres. destruct hres as [RES' [RES_RQ_RES' hres']].
+             inversion res_qs as [res_qs'].
+             iSpecialize ("IH" $! RES' LRES' eq_refl hres' qs' hqs').
+             rewrite {3}/list_map. do 7 tp_pure ; fold list_map.
+             tp_bind (list_map f' _).
+             iSpecialize ("IH" with "rhs").
+             wp_bind (list_map f _).
+             iApply (wp_strong_mono'' with "IH").
+             iIntros "%vRES (%vRES' & rhs & %hRES)".
+             rewrite /list_cons /= ; tp_pures ; wp_pures ; rewrite -/list_cons.
+             tp_bind (f' _) ; wp_bind (f _).
+             iPoseProof (ff_pweq _ Q RQ) as "hQ".
+             iSpecialize ("hQ" with "rhs").
+             iApply (wp_strong_mono'' with "hQ").
+             iIntros "%vQ (%vQ' & rhs & %hQQ') /=".
+             rewrite /list_cons /= ; tp_pures ; wp_pures ; rewrite -/list_cons.
+             iFrame. iPureIntro. intros. simplify_eq.
+             specialize (hQQ' eq_refl). specialize (hRES eq_refl). subst. done.
+         -
+           (* if RES is not a list of the same length as the inputs qs, we should get a contradiction out of safety. *)
+           iRevert "rhs".
+           iAssert
+             (⤇ fill K (list_map f' qs) -∗
+              WP list_map f qs {{ v, ∃ v' : val,
+                      ⤇ fill K v'
+                      ∗ ⌜v = RES → ∃ Lv : list val, is_list Lv RES ∧ length Lv = length QS⌝ }})%I as "HH".
+           2: { iIntros "rhs". iSpecialize ("HH" with "rhs"). iApply (wp_strong_mono'' with "HH").
+                iIntros "%v (%v' & rhs & %Lv)".
+                iFrame. iIntros "%h". exfalso.
+                apply HRES in Lv. all: assumption.
+           }
+           iIntros "rhs". clear HRES.
+           iInduction QS as [ | Q QS'] "IH" forall (qs hqs K RES) ; simpl in hqs.
+           + subst. rewrite /list_map. tp_pures ; wp_pures. iFrame. iIntros "!> %". subst. iExists []. done.
+           + destruct hqs as (qs' & hqs & hqs').
+             rewrite {4}/list_map. wp_pures.
+             rewrite hqs.
+             do 4 wp_pure _. fold list_map.
+             rewrite {3}/list_map. do 7 tp_pure ; fold list_map.
+             (* To use the IH we need to conjure up the result corresponding to the recursive call. *)
+             destruct_decide (make_decision (∃ RQ RQS' : val, RES = InjRV (RQ, RQS'))) as HRES.
+             * destruct HRES as (RQ & RQS' & HRES).
+               iSpecialize ("IH" $! qs' hqs' _ RQS'). tp_bind (list_map f' _). iSpecialize ("IH" with "rhs").
+               wp_bind (list_map f _).
+               iApply (wp_strong_mono'' with "IH").
+               iIntros "%vRES (%vRES' & rhs & %hRES)".
+               rewrite /list_cons /= ; tp_pures ; wp_pures ; rewrite -/list_cons.
+               tp_bind (f' _) ; wp_bind (f _).
+               iApply (wp_strong_mono'' $! (f_safe _)). iIntros.
+               iMod (f'_safe with "rhs") as "(% & rhs)". simpl. tp_pures. wp_pures.
+               rewrite /list_cons /= ; tp_pures ; wp_pures ; rewrite -/list_cons.
+               iFrame. iPureIntro. intros. simplify_eq.
+               specialize (hRES eq_refl). destruct hRES as (Lv' & Lv_RQS' & Lv_QS').
+               eexists (RQ :: Lv'). simpl. intuition eauto.
+             *
+               (* by safety of list_map and f we should be able to get a contradiction now even w/o the IH. *)
+               iClear "IH".
+               iRevert "rhs".
+               iAssert
+                 (⤇ fill K (list_cons (f' (Fst (Q, qs')%V)) (list_map f' qs')) -∗
+                  WP list_cons (f (Fst (Q, qs')%V)) (list_map f qs')
+                    {{ v, ∃ v' : val, ⤇ fill K v' ∗ ⌜v = RES → ∃ RQ RQS' : val, RES = InjRV (RQ, RQS')⌝ }})%I as "HH".
+               2: { iIntros "rhs". iSpecialize ("HH" with "rhs"). iApply (wp_strong_mono'' with "HH").
+                    iIntros "%v (%v' & rhs & %Lv)". iFrame. iPureIntro. intros ->.
+                    specialize (Lv eq_refl). done.
+               }
+               iIntros "rhs". clear HRES.
+               pose proof wp_list_map_safe as hh.
+               pose proof (spec_list_map_safe f' f'_safe) as hh'.
+               tp_bind (list_map _ _). iMod ((hh' _ _) with "rhs") as "(%v' & rhs) /=". 1: done. tp_pures. tp_bind (f' _).
+               iMod (f'_safe _ _ with "rhs") as "(% & rhs) /=". rewrite {1}/list_cons. tp_pures.
+               wp_bind (list_map _ _).
+               pose proof (hh f f_safe) as h.
+               iApply (wp_strong_mono'' $! (h _ _ _)). iIntros. wp_pures. wp_bind (f _).
+               iApply (wp_strong_mono'' $! (f_safe _)). iIntros. rewrite /list_cons. wp_pures.
+               iFrame. iPureIntro. intros <-. eauto.
+               Unshelve. 2: eauto.
+       Qed.
+
+       (* (map f qs) and (map f' qs) are point-wise equal for any list qs. *)
+       (* different proof strategy: start the induction before casing and only get two cases instead of the full list of results *)
+       Goal (∀ K RES (qs : val) QS (hqs : is_list QS qs), ⊢ ⤇ fill K (list_map f' qs) -∗
+                  WP (list_map f qs)
+                    {{ v , ∃ v' : val , ⤇ fill K (Val v') ∗ ⌜v = RES → v' = RES⌝ }}).
+
+         intros. iIntros "rhs".
+         iInduction QS as [ | Q QS'] "IH" forall (RES qs hqs K) ; simpl in hqs.
+         (* we have to conjure up the intermediate results that got collected into RES *)
+         - subst. rewrite /list_map. tp_pures. wp_pures. iFrame. done.
+         -
+           destruct hqs as (qs' & hqs & hqs').
+           rewrite {4}/list_map. wp_pures.
+           rewrite hqs.
+           do 4 wp_pure _. fold list_map.
+           rewrite {3}/list_map. do 7 tp_pure ; fold list_map.
+           (* To use the IH we need to conjure up the result corresponding to the recursive call. *)
+           destruct_decide (make_decision (∃ RQ RQS' : val, RES = InjRV (RQ, RQS'))) as HRES.
+           + destruct HRES as (RQ & RQS' & HRES).
+             iSpecialize ("IH" $! RQS' qs' hqs' _). tp_bind (list_map f' _). iSpecialize ("IH" with "rhs").
+             wp_bind (list_map f _).
+             iApply (wp_strong_mono'' with "IH").
+             iIntros "%vRES (%vRES' & rhs & %hRES)".
+             rewrite /list_cons /= ; tp_pures ; wp_pures ; rewrite -/list_cons.
+             tp_bind (f' _) ; wp_bind (f _).
+             iPoseProof (ff_pweq _ Q RQ) as "hQ".
+             iSpecialize ("hQ" with "rhs").
+             iApply (wp_strong_mono'' with "hQ").
+             iIntros "%vQ (%vQ' & rhs & %hQQ') /=".
+             rewrite /list_cons /= ; tp_pures ; wp_pures ; rewrite -/list_cons.
+             iFrame. iPureIntro. intros. simplify_eq.
+             specialize (hQQ' eq_refl). specialize (hRES eq_refl). subst. done.
+           +
+             (* by safety of list_map and f we should be able to get a contradiction now even w/o the IH. *)
+             iClear "IH".
+             iRevert "rhs".
+             iAssert
+               (⤇ fill K (list_cons (f' (Fst (Q, qs')%V)) (list_map f' qs')) -∗
+                WP list_cons (f (Fst (Q, qs')%V)) (list_map f qs')
+                  {{ v, ∃ v' : val, ⤇ fill K v' ∗ ⌜v = RES → ∃ RQ RQS' : val, RES = InjRV (RQ, RQS')⌝ }})%I as "HH".
+             2: { iIntros "rhs". iSpecialize ("HH" with "rhs"). iApply (wp_strong_mono'' with "HH").
+                  iIntros "%v (%v' & rhs & %Lv)". iFrame. iPureIntro. intros ->.
+                  specialize (Lv eq_refl). done.
+             }
+             iIntros "rhs". clear HRES.
+             pose proof wp_list_map_safe as hh.
+             pose proof (spec_list_map_safe f' f'_safe) as hh'.
+             tp_bind (list_map _ _). iMod ((hh' _ _) with "rhs") as "(%v' & rhs) /=". 1: done. tp_pures. tp_bind (f' _).
+             iMod (f'_safe _ _ with "rhs") as "(% & rhs) /=". rewrite {1}/list_cons. tp_pures.
+             wp_bind (list_map _ _).
+             pose proof (hh f f_safe) as h.
+             iApply (wp_strong_mono'' $! (h _ _ _)). iIntros. wp_pures. wp_bind (f _).
+             iApply (wp_strong_mono'' $! (f_safe _)). iIntros. rewrite /list_cons. wp_pures.
+             iFrame. iPureIntro. intros <-. eauto.
+             Unshelve. 2: eauto.
+       Qed.
+
+     End concrete_example.
+   *)
+  (* END TEMP COMMENT *)
+
+  (* list_map offline XC from online, but pointwise *)
+  Lemma exact_cache_dipr_offline_map_pw (M : val) DB (dDB : Distance DB) (qs : list nat) (QS : val) (is_qs : is_list qs QS)
+    ε δ (εpos : 0 <= ε) (δpos : 0 <= δ)
+    (M_dipr : Forall (λ q : nat, ⊢ wp_diffpriv_pw (M #q) ε δ dDB) qs)
+    :
+    let k := size ((list_to_set qs) : gset _) in
+    ⊢ wp_diffpriv_pw (exact_cache_offline_map M QS) (k*ε) (k*δ) dDB.
+  Proof with (tp_pures ; wp_pures).
+    iIntros (k K c db db' adj) "[rhs [ε δ]] %RES".
+    rewrite {2}/exact_cache_offline_map...
+    rewrite /exact_cache_offline_map...
+    tp_bind (online_xcache _ _). wp_bind (online_xcache _ _).
+    iPoseProof (oxc_spec0_pw M _ _ _ _) as "oXC" => //.
+    iSpecialize ("oXC" with "rhs").
+    iApply (wp_strong_mono'' with "oXC").
+    iIntros "%f (%f' & rhs & %F & %G & F & FG & #cached & #fresh) /="...
+    (* strengthen the postcondition with the resources for the cache & size information for the credits *)
+    cut
+      ( ∀ K,
+                ↯m (c * (k * ε)) ∗ ↯ (c * (k * δ)) ∗
+                □ oxc_spec0_pw_cached f f' G ∗
+                □ oxc_spec0_pw_fresh M c dDB f f' F G ∗
+                ⤇ fill K (list_map f' QS) ∗
+                F ∅ ∗
+                □ (∀ A : gmap nat val, F A ∗-∗ G A A)
+                -∗
+               WP list_map f QS
+                 {{ vl,
+                   ∃ (vr : val) (lvl lvr : list val) cache_qs_l cache_qs_r,
+                     ⌜is_list lvl vl⌝ ∗ ⌜is_list lvr vr⌝ ∗
+                     ⌜dom cache_qs_l = list_to_set qs⌝ ∗
+                     ⌜dom cache_qs_r = list_to_set qs⌝ ∗
+                     ⤇ fill K vr ∗
+                     G cache_qs_l cache_qs_r ∗
+                     (⌜vl = RES⌝ -∗
+                     (⌜cache_qs_l = cache_qs_r⌝ ∗ ⌜vr = RES⌝)) }} ).
+    { intros h. intros. iPoseProof (h with "[-]") as "h" => //.
+      1: iFrame ; repeat iSplit ; try done.
+      iApply (wp_strong_mono'' with "h").
+      iIntros (?) "(% & % & % & % & % & % & % & % & % & rhs & G & F_heq)" ; subst ; iFrame.
+      iIntros "%eqres". iDestruct ("F_heq" $! eqres) as "[-> ->]". done.
+    }
+    Unshelve. 2: eauto.
+    iInduction qs as [|q' qs'] "IH" forall (RES QS is_qs).
+    - iIntros (K'). iIntros "(ε & δ & #? & #? & rhs & F & FG)".
+      simpl in is_qs. subst. rewrite /list_map... simplify_eq.
+      iDestruct ("FG" with "F") as "G".
+      iFrame. iExists [],[].
+      iModIntro.
+      repeat iSplit ; try done.
+    - iIntros (K').
+      iIntros "(ε & δ & #cached & #fresh & rhs & F & #FG)".
+      set (qs := q' :: qs').
+      rewrite {4}/list_map... rewrite -/list_map.
+      rewrite {3}/list_map... rewrite -/list_map.
+
+      destruct is_qs as (QS' & -> & is_qs')...
+      destruct (Forall_cons_1 _ _ _ M_dipr) as [M_dipr_q' M_dipr_qs'].
+      assert (0 <= dDB db db') by apply distance_pos.
+      destruct_decide (make_decision (∃ RQ RQS' : val, RES = InjRV (RQ, RQS'))) as HRES.
+{
+      tp_bind (list_map f' _) ; wp_bind (list_map f _).
+      destruct HRES as (RQ & RQS' & HRES).
+      iSpecialize ("IH" $! M_dipr_qs' RQS' QS' is_qs' _).
+      destruct_decide (make_decision (q' ∈ qs')) as cache_q'.
+      + subst k.
+        assert (list_to_set qs = list_to_set qs') as ->.
+        { subst qs. simpl. set_solver. }
+        iSpecialize ("IH" with "[$]").
+        iApply (wp_strong_mono'' with "IH").
+        iIntros "%vl (%vr & %lvl & %lvr & %cache_qs'_l & %cache_qs'_r & %is_vl & %is_vr & %dom_cache_qs'_l & %dom_cache_qs'_r & rhs & G & %eqv)".
+        iSimpl in "rhs"... tp_bind (f' _) ; wp_bind (f _).
+        unshelve iSpecialize ("cached" $! q' cache_qs'_l cache_qs'_r _ _ _ with "G rhs").
+        { rewrite dom_cache_qs'_l. set_solver. }
+        { rewrite dom_cache_qs'_r. set_solver. }
+        iApply (wp_strong_mono'' with "cached").
+        iIntros "/= %vq'_l (%vq'_r & G & rhs & %cache_q'')".
+        rewrite /list_cons...
+        iFrame. iModIntro. iPureIntro. simpl.
+        eexists (vq'_l :: lvl), (vq'_r :: lvr). intuition auto.
+        * simpl. eexists _. intuition auto.
+        * simpl. eexists _. intuition auto.
+        * set_solver.
+        * set_solver.
+        * subst. simplify_eq. destruct (eqv eq_refl) as [-> ->]. reflexivity.
+        * subst. simplify_eq. destruct (eqv eq_refl) as [-> ->]. simplify_eq. reflexivity.
+      + set (k' := size (list_to_set qs' : gset _)).
+        assert ((k = 1 + k')%nat) as ->.
+        { subst k. simpl list_to_set. rewrite size_union. 1: rewrite size_singleton ; lia. set_solver. }
+        replace (c * ((1 + k')%nat * δ)) with (c * δ + c * (k' * δ)).
+        2:{ real_solver_partial. rewrite plus_INR INR_1. field. }
+        replace (c * ((1 + k')%nat * ε)) with (c * ε + c * (k' * ε)).
+        2:{ real_solver_partial. rewrite plus_INR INR_1. field. }
+        iDestruct (ecm_split with "ε") as "[ε k'ε]".
+        2: real_solver. 1: repeat real_solver_partial => //.
+        iDestruct (ec_split with "δ") as "[δ k'δ]".
+        2: real_solver. 1: repeat real_solver_partial => //.
+        iSpecialize ("IH" with "[-ε δ]") ; [iFrame ; repeat iSplit ; done|].
+        iApply (wp_strong_mono'' with "IH").
+        iIntros "%vqs'_l (%vqs'_r & %lvqs'_l & %lvqs'_r & %cache_qs'_l & %cache_qs'_r & %is_vqs'_l & %is_vqs'_r & %dom_cache_qs'_l & %dom_cache_qs'_r & rhs & G & %pweq_vqs')".
+        iSimpl in "rhs"... tp_bind (f' _) ; wp_bind (f _).
+        unshelve iSpecialize ("fresh" $! q' cache_qs'_l cache_qs'_r ε δ _ _ _ M_dipr_q' with "ε δ G rhs").
+        1: rewrite dom_cache_qs'_l ; set_solver.
+        1: rewrite dom_cache_qs'_r ; set_solver.
+        iSpecialize ("fresh" $! RQ).
+        iApply (wp_strong_mono'' with "fresh").
+        iIntros "/= %vq'_l (%vq'_r & G & rhs & pweq_fresh)".
+        rewrite /list_cons...
+        iFrame "rhs". iModIntro. simpl.
+        iExists (vq'_l :: lvqs'_l), (vq'_r :: lvqs'_r).
+        iExists (<[q':=vq'_l]> cache_qs'_l), (<[q':=vq'_r]> cache_qs'_r).
+        repeat iSplit.
+        * iPureIntro. simpl. eexists _. intuition auto.
+        * iPureIntro. simpl. eexists _. intuition auto.
+        * iPureIntro. set_solver.
+        * iPureIntro. set_solver.
+        * iFrame.
+        * iIntros "%". iSplit.
+          -- simplify_eq. destruct pweq_vqs' => //. simplify_eq.
+             iDestruct ("pweq_fresh" with "[] G") as "[F %eq_vq'_r]".
+             1: done. simplify_eq. done.
+          -- simplify_eq. destruct pweq_vqs' => //. simplify_eq.
+             iDestruct ("pweq_fresh" with "[] G") as "[F %eq_vq'_r]".
+             1: done. simplify_eq. done.
+}
+{
+  iClear "IH ε δ".
+  iRevert "rhs".
+  iAssert (
+              (* ↯m (c * (k * ε)) ∗ ↯ (c * (k * δ)) ∗ *)
+              (* □ oxc_spec0_pw_cached f f' G ∗
+                 □ oxc_spec0_pw_fresh M c dDB f f' F G ∗ *)
+              ⤇ fill K' (list_cons (f' (Fst (#q', QS')%V)) (list_map f' QS')) -∗
+              F ∅
+              (* □ (∀ A : gmap nat val, F A ∗-∗ G A A) *)
+              -∗
+              WP list_cons (f (Fst (#q', QS')%V)) (list_map f QS')
+                {{ vl,
+                     ∃ (vr : val) (lvl lvr : list val) cache_qs_l cache_qs_r,
+                       ⌜is_list lvl vl⌝ ∗ ⌜is_list lvr vr⌝ ∗
+                       ⌜dom cache_qs_l = list_to_set qs⌝ ∗
+                       ⌜dom cache_qs_r = list_to_set qs⌝ ∗
+                       ⤇ fill K' vr ∗
+                       G cache_qs_l cache_qs_r ∗
+                       (⌜vl = RES → ∃ RQ RQS' : val, RES = InjRV (RQ, RQS')⌝
+                        (* (⌜cache_qs_l = cache_qs_r⌝ ∗ ⌜vr = RES⌝) *)) }} )%I as "HH".
+  2: { iIntros "rhs". iSpecialize ("HH" with "rhs F"). iApply (wp_strong_mono'' with "HH").
+       iIntros "%v (%v' &% &% &% &% &% &% &% &% & rhs & G & %Lv)". iFrame. iPureIntro. simpl.
+       eexists _,_.
+       repeat split ; try done.
+       - exfalso. eauto.
+       - exfalso. eauto.
+  }
+      tp_bind (list_map f' _) ; wp_bind (list_map f _).
+
+
+}
+
+  Qed.
+
+  (* offline XC from online, but pointwise *)
+  Lemma exact_cache_dipr_offline_pw (M : val) DB (dDB : Distance DB) (qs : list nat) (QS : val) (is_qs : is_list qs QS)
+    ε δ (εpos : 0 <= ε) (δpos : 0 <= δ)
+    (M_dipr : Forall (λ q : nat, ⊢ wp_diffpriv_pw (M #q) ε δ dDB) qs)
+    :
+    let k := size ((list_to_set qs) : gset _) in
+    ⊢ wp_diffpriv_pw (exact_cache_offline M QS) (k*ε) (k*δ) dDB.
+  Proof with (tp_pures ; wp_pures).
+    iIntros (k K c db db' adj) "[rhs [ε δ]] %RES".
+    rewrite {2}/exact_cache_offline...
+    rewrite /exact_cache_offline...
+    tp_bind (online_xcache _ _). wp_bind (online_xcache _ _).
+    iPoseProof (oxc_spec0_pw M _ _ _ adj with "rhs") as "oXC" => //.
+    iApply (wp_strong_mono'' with "oXC").
+    iIntros "%f (%f' & rhs & %F & F & cached & fresh) /="...
+    set (exact_cache_offline_body (f : val) := (λ: "acc" "q", list_cons (f "q") "acc")%V).
+    rewrite -!/(exact_cache_offline_body _).
+    revert RES qs QS is_qs k M_dipr.
+    cut
+      (∀ (RES : val) (qs : list nat)
+         (qs_pre qs' : list nat) (QS' : val)
+         (acc : val) cache_map,
+          qs = qs_pre ++ qs' →
+          dom cache_map = list_to_set qs_pre →
+          dom cache_map ∪ list_to_set qs' = list_to_set qs →
+          is_list qs' QS' →
+          Forall (λ q : nat, ⊢ wp_diffpriv_pw (M #q) ε δ dDB) qs →
+          let k := size (list_to_set qs : gset nat) in
+          let k' := size cache_map in
+          {{{
+                ↯m (c * ((k - k') * ε)) ∗ ↯ (c * ((k - k') * δ)) ∗
+                □ oxc_spec0_cached f f' F ∗
+                □ oxc_spec0_pw_fresh M c dDB f f' F ∗
+                ⤇ fill K (list_fold (exact_cache_offline_body f') acc QS') ∗
+                F cache_map
+          }}}
+            list_fold (exact_cache_offline_body f) acc QS'
+            {{{ vl, RET vl ; ∃ (vr : val), ⤇ fill K vr ∗ (⌜vl = RES → vr = RES⌝) }}}
+      ).
+    {
+      intros h. intros. iApply (h RES qs [] qs QS _ ∅ with "[-]") => //.
+      1: set_solver.
+      2:{ iNext. iIntros "%vl h". iApply "h". }
+      iFrame. rewrite map_size_empty. rewrite Rminus_0_r. subst k. simpl. iFrame.
+    }
+    iLöb as "IH".
+    iIntros (RES qs qs_pre qs' QS' acc cache qs_pre_qs' dom_cache_pre dom_cache_qs'_qs is_qs'
+               M_dipr φ) "(ε & δ & #cached & #fresh & rhs & F) hφ".
+    set (k := size (list_to_set qs : gset nat)).
+    set (k' := size cache).
+    rewrite {4}/exact_cache_offline_body/list_fold... rewrite -!/(exact_cache_offline_body _) -/list_fold.
+    destruct qs' as [|q' qs''] eqn:qs'_qs''.
+    1:{ rewrite is_qs'. rewrite {3}/exact_cache_offline_body/list_fold... iApply "hφ". iExists _. iFrame => //. }
+    destruct is_qs' as (QS'' & -> & is_qs'')...
+    rewrite -!/(exact_cache_offline_body _) -/list_fold.
+    rewrite qs_pre_qs' in M_dipr.
+    destruct ((proj1 (List.Forall_app _ _ _)) M_dipr) as [M_dipr_qs_pre M_dipr_qs'].
+    destruct (Forall_cons_1 _ _ _ M_dipr_qs') as [M_dipr_q' M_dipr_qs''].
+    assert (0 <= dDB db db') by apply distance_pos.
+    destruct (cache !! q') eqn:cache_q' => /=.
+    - opose proof (elem_of_dom_2 _ _ _ cache_q') as h...
+      rewrite /exact_cache_offline_body...
+      tp_bind (f' _) ; wp_bind (f _).
+      iCombine "cached" as "h".
+      iSpecialize ("h" $! q' cache _ h with "F rhs").
+      iApply (wp_strong_mono'' with "h").
+      iIntros "/= %v' (F & rhs & %cache_q'')".
+      assert (v = v') as <-. { rewrite cache_q' in cache_q''. inversion cache_q''. done. }
+      rewrite /list_cons...
+      rewrite -!/(exact_cache_offline_body _) -/list_fold.
+      iSpecialize ("IH" $! RES qs (qs_pre ++ [q']) qs'' QS'' (InjRV (v, acc)) cache).
+      unshelve iApply ("IH" $! _ _ _ _ _ _ with "[ε δ rhs F]") => //.
+      1: subst ; by rewrite cons_middle assoc.
+      all: subst ; try assumption.
+      1,2: set_solver. iFrame. iSplit ; done.
+    - opose proof (not_elem_of_dom_2 _ _ cache_q') as h...
+      assert ((c * ((k - k') * ε)) = (c * (k - (k'+1)) * ε + c * ε)) as -> by lra.
+      assert ((c * ((k - k') * δ)) = (c * (k - (k'+1)) * δ + c * δ)) as -> by lra.
+      assert (0 <= k - (k' + 1)).
+      {
+        subst. subst k k'. apply Rle_0_le_minus.
+        rewrite -dom_cache_qs'_qs.
+        replace (size cache) with (size (dom cache)) by apply size_dom.
+        rewrite dom_cache_pre.
+        replace 1 with (INR 1) by auto.
+        replace 1%nat with (size (list_to_set [q'] : gset nat)).
+        2:{ cbn. rewrite union_empty_r_L. apply size_singleton. }
+        rewrite -plus_INR.
+        rewrite -size_union.
+        2: set_solver.
+        rewrite (list_to_set_cons _ qs''). simpl.
+        apply le_INR.
+        apply subseteq_size. set_solver.
+      }
+      iDestruct (ecm_split with "ε") as "[kε ε]".
+      2: real_solver. 1: repeat real_solver_partial => //.
+      iDestruct (ec_split with "δ") as "[kδ δ]".
+      2: real_solver. 1: repeat real_solver_partial => //.
+      rewrite /exact_cache_offline_body...
+      tp_bind (f' _) ; wp_bind (f _).
+      iCombine "fresh" as "h".
+      iSpecialize ("h" $! q' cache ε δ _ h M_dipr_q' with "ε δ F rhs").
+      (* need to guess the result of (f #q') here... *)
+      destruct_decide (make_decision (∃ RQ' RQS' : val, RES = InjRV (RQ', RQS'))) as HRES.
+      {
+        destruct HRES as (RQ' & RQS' & RES_QQS').
+        iSpecialize ("h" $! RQ').
+      iApply (wp_strong_mono'' with "h").
+      iIntros "%vq' Hres".
+      (* postponing these two lines until we need them *)
+      (* iSpecialize ("Hres" $! _).
+         iDestruct "Hres" as "(F & rhs & %cache_q'') /=". *)
+      rewrite /list_cons... rewrite -/list_cons.
+      iSpecialize ("IH" $! RES qs (qs_pre ++ [q']) qs'' QS'' (InjRV (vq', acc)) (<[q':=vq']> cache)).
+      unshelve iSpecialize ("IH" $! _ _ _ _ _) => //.
+      1: subst ; by rewrite cons_middle assoc.
+      1: { simplify_eq. rewrite list_to_set_app_L. rewrite -dom_cache_pre.
+           simpl. pose proof (dom_insert_L cache q' (vq' : val)) as ->. set_solver. }
+      1: set_solver. 1: done. 1: { rewrite qs_pre_qs'. done. }
+      iSpecialize ("IH" with "[kε kδ rhs $F]") => //.
+      2: iApply "IH" => //. iFrame.
+      iSplitL "kε" ; [|iSplitL "kδ"]. 3: iSplit ; done.
+      + iApply ecm_eq. 2: iFrame. real_solver_partial.
+        subst k. simpl. subst k'.
+        replace (INR $ size (<[q' := vq']> cache)) with (size cache + 1).
+        1: done.
+        rewrite map_size_insert_None => //. qify_r ; zify_q. lia.
+      + iApply ec_eq. 2: iFrame. real_solver_partial.
+        subst k. simpl. subst k'.
+        replace (INR $ size (<[q' := vq']> cache)) with (size cache + 1).
+        1: done.
+        rewrite map_size_insert_None => //. qify_r ; zify_q. lia.
+        Unshelve.
+simpl in *. simplify_eq.
+
+        1: {  }
+        all: try (subst ; done).
+        3,4: set_solver.
+        1: subst ; by rewrite cons_middle assoc.
+        all: subst ; assumption || set_solver.
+
+  Qed.
 
   (* Does it make sense to store f' (the result of the rhs) in F? Probably not. *)
   Lemma oxc_spec2 (M : val) `(dDB : Distance DB) (db db' : DB) (adj : dDB db db' <= 1) K ε δ :
